\documentclass{article}

\usepackage[most]{tcolorbox}
\usepackage{physics}
\usepackage{graphicx}
\usepackage{float}
\usepackage{amsmath}
\usepackage{amssymb}


\usepackage[utf8]{inputenc}
\usepackage[a4paper, margin=1in]{geometry} % Controla los márgenes
\usepackage{titling}

\title{Parcial \#2 }
\author{Manuel Garcia.}
\date{\today}

\renewcommand{\maketitlehooka}{%
  \centering
  \vspace*{0.05cm} % Espacio vertical antes del título
}

\renewcommand{\maketitlehookd}{%
  \vspace*{2cm} % Espacio vertical después de la fecha
}

\newcommand{\caja}[3]{%
  \begin{tcolorbox}[colback=#1!5!white,colframe=#1!25!black,title=#2]
    #3
  \end{tcolorbox}%
}

\begin{document}
\maketitle

\section{}
\begin{gather}
  U ^ {\mu} \partial _{\mu} \langle V, W \rangle = \langle U ^ {\mu} \grad _{\mu} V, W \rangle + \langle V, U ^ {\mu} \grad _{\mu}  W \rangle \\
  U ^ {\mu } \partial _{\mu} (g _{\lambda \beta} V ^ {\alpha}W ^ {\beta}) = U ^ {\mu} (\partial _{\mu} g _{\lambda\beta} ) V ^ {\lambda} W ^ {\beta} + U ^ {\mu} g _{\lambda\beta} (\partial _{\mu} V ^ {x })W ^ {\beta} + U ^ {\mu} g _{\lambda\beta} (\partial _{\mu} W ^ {\beta})V ^ {\lambda} \\
  \text{Tenemos que: }\\
  \grad _{\mu} g _{\lambda\beta} - \Gamma _{\mu\lambda} ^ {\rho} g _{\rho\beta} - \Gamma _{\mu\beta} g _{\lambda \rho}  \qquad \qquad \grad _{\mu} T ^ {\lambda} = \partial _{\mu} T ^ {\lambda} + \Gamma _{\rho\mu} ^ {\lambda} T ^ {\rho}\\
  \text{Entonces: }\\
  = U ^ {\mu}(\grad _{\mu} g _{\lambda\beta} + \Gamma _{\mu\lambda} ^ {\rho} g _{\rho\beta} + \Gamma _{\mu\beta} g _{\lambda \rho})V ^ {\lambda}W ^ {\beta} + U ^ {\mu}g _{\lambda\beta} (\grad _{\mu} V ^ {\lambda} - \Gamma _{\rho\mu} V ^ {\rho})W ^ {\beta} + U ^ {\mu} g _{\lambda\beta} (\grad _{\mu} W ^ {\beta} - \Gamma _{\rho\mu} ^ {\beta} W ^ {\rho})V ^ {\lambda}\\
  = U ^ {\mu} (g _{\lambda\beta} (\grad _{\mu } V ) ^ {\lambda}W ^ {\beta} + g _{\lambda\beta} V ^ {\lambda} (\grad _{\mu} W ^ {\beta})) \\
  = \langle U ^ {\mu} \grad _{\mu}  V , W \rangle + \langle V, U ^ {\mu} \grad _{\mu} W \rangle
\end{gather}


%%%%%%%%%%%%%%%%%%%%%%%%%%%%%%%%%%%%%%%%%%%%%%%%%%%%%%%%%%%%%%%%%%%


\section{}
\begin{gather}
  \omega = 4xydx + (x^2 - 5) dy \qquad \quad \beta = e ^ {2xy } dx - dy \\
  x = 2 \frac{d  }{d x } + y \frac{d  }{d y }
\end{gather}

\begin{itemize}
  \item 
  \begin{align*}
    d\omega &= d(4xy dx ) + d((x^2-5)dy)\\
       &= (4ydx + 4x dy) \land dx + (2x dx)\land dy \\
       &= (-4x + 2x ) (dx \land dy)
  \end{align*}
  \item 
  \begin{align*}
    d\beta &= d(e ^ {2y } dx ) + d(-dy)\\
       &= (2x e ^ {2xy }dy + 2y e ^ {2xy }dx )\land dx \\
       &= 2x e ^ {2xy } dy \land dx 
  \end{align*}
  \item 
  \begin{align*}
    \omega \land \beta &= (4xy dx + (x^2 - 5) dy ) \land (e ^ {2xy }dx - dy ) \\
    &= 4xydx\land(e ^ {2xy }dx - dy ) + (x^2 - 5) dy \land (e ^ {2xy }dx - dy ) \\
    &= - 4xy dx \land dy + (x^2 - 5) e ^ {2xy }dy\land dx \\
    &= -(4xy + (x^2 - 5)e ^ {2xy })dx \land dy 
  \end{align*}
  \item 
  \begin{align*}
    i_x d\beta &= i _{x } (2x e ^ {2xy } dy \land dx) = 2x e ^ {2xy } (dy(y \frac{\partial  }{\partial y })\otimes dx - dx (2 \frac{\partial  }{\partial x }))\otimes dy \\
          &= 2xy e ^ {2xy }dy - 4 x e ^ {2xy }dy 
  \end{align*}
  \item 
  \begin{align*}
    d\beta \land \omega &= (2x e ^ {2xy } dy \land dx ) \land (4xy dx + (x^2 - 5) dy ) \\
    &= 2x e ^ {2xy }(x^2 - 5 )dy \land dx \land dy = 0 
  \end{align*}
  \item 
  \begin{align*}
    d\omega \land \beta = (-2x dx \land dy ) \land (e ^ {2xy } dx - dy ) = 0 
  \end{align*}
\end{itemize}

%%%%%%%%%%%%%%%%%%%%%%%%%%%%%%%%%%%%%%%%%%%%%%%%%%%%%%%%%%%%%%%

\section{}
\begin{align*}
  \Delta \Gamma _{\beta\gamma} ^ {\alpha} &= \Gamma _{\beta\gamma} ^ {\alpha} - \bar \Gamma _{\beta\gamma} ^ {\alpha} \quad \in \mathcal{T}(M) \\
  (\Delta \Gamma _{\beta\gamma}  ^ {\alpha} )' &= (\Gamma _{\beta\gamma}  ^ {\alpha})' - (\bar \Gamma _{\beta\gamma} ^ {\alpha})'\\
  &= \left(\frac{ y ^ {\alpha} }{\partial x ^ {\beta}} \frac{\partial x ^ {\alpha} }{\partial y ^ {\nu}} \frac{\partial y ^ {\sigma} }{\partial y ^ {\mu}} \Gamma _{\alpha\sigma} ^ {\beta} - \frac{ y ^ {\alpha} }{\partial x ^ {\beta}} \frac{\partial x ^ {\alpha} }{\partial y ^ {\nu}} \frac{\partial y ^ {\sigma} }{\partial y ^ {\mu}} \bar\Gamma _{\alpha\sigma} ^ {\beta}\right) \\
  &=\frac{ y ^ {\alpha} }{\partial x ^ {\beta}} \frac{\partial x ^ {\alpha} }{\partial y ^ {\nu}} \frac{\partial y ^ {\sigma} }{\partial y ^ {\mu}} (\Gamma _{\alpha\sigma}  ^ {\beta} - \bar \Gamma _{\alpha\sigma}  ^ {\beta})\\
  &= \frac{ y ^ {\alpha} }{\partial x ^ {\beta}} \frac{\partial x ^ {\alpha} }{\partial y ^ {\nu}} \frac{\partial y ^ {\sigma} }{\partial y ^ {\mu}}\Delta \Gamma _{\alpha\sigma}  ^ {\beta}
\end{align*}

%%%%%%%%%%%%%%%%%%%%%%%%%%%%%%%%%%%%%%%%%%%%%%%%%%%%%%%%%%%%%%%

\section{}


%%%%%%%%%%%%%%%%%%%%%%%%%%%%%%%%%%%%%%%%%%%%%%%%%%%%%%%%%%%%%%%

\section{}
\begin{gather*}
  R _{\mu\nu\alpha\beta}  = R _{\mu\alpha} g _{\nu\beta} - R _{\mu\beta} g _{\nu\alpha} + R _{\nu\beta} g _{\mu\alpha} - R _{\nu\alpha} g _{\mu\beta} + \frac{R }{2 } (g _{\mu\beta} g _{\nu\alpha } - g _{\mu\alpha} g _{\nu\beta} ) \\
  g ^ {\nu\beta} R _{\mu\nu\alpha\beta}  = R _{\mu\alpha}  = R _{\mu\alpha} g _{\nu\beta} g ^ {\nu\beta} - R _{\mu\beta} g _{\nu\alpha} g ^ {\nu\beta} + R _{\nu\beta} g ^ {\nu\beta} g _{\mu\alpha} - R _{\nu\alpha} g ^ {\nu\beta} g _{\mu\alpha} + \frac{R }{2} ( g _{\mu\beta} g _{\nu\alpha} g ^ {\nu\beta}- g _{\mu\alpha}  g _{\nu\beta} g ^ {\nu\beta})\\
  = R _{\mu\alpha}  g _\nu^\nu - R _{\mu\beta} g _\alpha^\beta + R g _{\mu\alpha} - R _{\nu\alpha}  g _\mu^\nu + \frac{R }{2} (g _{\mu\beta} g_\alpha^\beta - g _{\mu\alpha} g_\nu^\nu) = R _{\mu\alpha} 
\end{gather*}

\end{document}
